@prefix dc:      <http://purl.org/dc/elements/1.1/> .
@prefix :        <http://iot.linkeddata.es/def/wot-mappings#> .
@prefix prov:    <http://www.w3.org/ns/prov#> .
@prefix geo:     <http://www.w3.org/2003/01/geo/wgs84_pos#> .
@prefix foaf:    <http://xmlns.com/foaf/0.1/> .
@prefix vann:    <http://purl.org/vocab/vann/> .
@prefix xml:     <http://www.w3.org/XML/1998/namespace> .
@prefix vs:      <http://www.w3.org/2003/06/sw-vocab-status/ns#> .
@prefix dcterms:  <http://purl.org/dc/terms/> .
@prefix wot:     <http://xmlns.com/wot/0.1/> .
@prefix rdfs:    <http://www.w3.org/2000/01/rdf-schema#> .
@prefix xsd:     <http://www.w3.org/2001/XMLSchema#> .
@prefix owl:     <http://www.w3.org/2002/07/owl#> .
@prefix rdf:     <http://www.w3.org/1999/02/22-rdf-syntax-ns#> .
@prefix saref:   <https://w3id.org/saref#> .
@prefix doap:    <http://usefulinc.com/ns/doap#> .

:isExecutedAfter
      a       owl:ObjectProperty ;
      rdfs:comment "Indicates which access mappings should be excuted before the one being subject of this property." ;
      rdfs:domain :AccessMapping ;
      rdfs:label "is executed after"@en ;
      rdfs:range :AccessMapping .

vs:term_status
      a       owl:AnnotationProperty .

:Mapping
      a       owl:Class ;
      rdfs:comment "An entity than indicates the relation between a given key (provided as structure data in an online resource) and the RDF property to which the values should be mapped and the target type of object. The RDF properties could be OWL object or datatype properties. The target object might be RDFS classes or datatypes."@en ;
      rdfs:label "Mapping"@en ;
      rdfs:subClassOf
              [ a       owl:Restriction ;
                owl:onProperty :key ;
                owl:someValuesFrom xsd:string
              ] ;
      rdfs:subClassOf
              [ a       owl:Restriction ;
                owl:minQualifiedCardinality
                        "1"^^xsd:nonNegativeInteger ;
                owl:onClass rdf:Property ;
                owl:onProperty :predicate
              ] ;
      owl:equivalentClass
              [ a       owl:Class ;
                owl:unionOf (:DatatypePropertyMapping :ObjectPropertyMapping)
              ] .

:mapsResourcesFrom
      a       owl:FunctionalProperty , owl:ObjectProperty ;
      rdfs:comment "Link from the access mapping to the specific endpoint in which the mappings (see hasMapping) indicated by the access mapping instance can be applied."@en ;
      rdfs:domain :AccessMapping ;
      rdfs:label "maps resources from"@en ;
      rdfs:range <http://iot.linkeddata.es/def/wot#Endpoint> .

:     a       owl:Ontology ;
      rdfs:comment "This ontology represent the mapping definitionts between WoT to allow interoperability in an IoT context based on VICINITY technological solutions."@en ;
      dc:publisher <http://www.oeg-upm.net/> ;
      dc:title "Vicinity WoT mappings model"@en ;
      dcterms:contributor <http://www.oeg-upm.net/index.php/en/universitystaff/402-fserena/> ;
      dcterms:creator <http://purl.org/net/mpoveda> , <http://www.garcia-castro.com/foaf.rdf#me> ;
      dcterms:license <http://purl.org/NET/rdflicense/cc-by4.0> ;
      vann:preferredNamespacePrefix
              "vcnt-map" ;
      vann:preferredNamespaceUri
              "http://iot.linkeddata.es/def/wot-mappings" ;
      owl:imports <http://iot.linkeddata.es/def/wot#> , <http://iot.linkeddata.es/def/core#> ;
      owl:versionInfo "0.0.2" .

:jsonPath
      a       owl:DatatypeProperty ;
      rdfs:comment "Express a pattern to select a set of efements of interest in a JSON document."@en ;
      rdfs:domain :Mapping ;
      rdfs:label "JSON path"@en ;
      rdfs:range xsd:string .

:targetDatatype
      a       owl:ObjectProperty ;
      rdfs:domain :DatatypePropertyMapping ;
      rdfs:label "target datatype"@en ;
      rdfs:range rdfs:Datatype .

:hasAccessMapping
      a       owl:ObjectProperty ;
      rdfs:comment "Link between a thing description and the access mapping that can be used to access the information provided in the endpoints exposes by such thing description. This class acts as an n-ary pattern linking the enpoints with the spedific mappings."@en ;
      rdfs:domain <http://iot.linkeddata.es/def/wot#ThingDescription> ;
      rdfs:label "has access mapping"@en ;
      rdfs:range :AccessMapping .

owl:DatatypeProperty
      a       owl:Class ;
      rdfs:isDefinedBy owl: ;
      rdfs:subClassOf rdf:Property .

:AccessMapping
      a       owl:Class ;
      rdfs:comment "This class allows the linking between one or more mappings that are executed against a given endpoint." ;
      rdfs:label "Access mapping"@en ;
      rdfs:subClassOf
              [ a       owl:Restriction ;
                owl:onClass <http://iot.linkeddata.es/def/wot#Endpoint> ;
                owl:onProperty :mapsResourcesFrom ;
                owl:qualifiedCardinality
                        "1"^^xsd:nonNegativeInteger
              ] ;
      rdfs:subClassOf
              [ a       owl:Restriction ;
                owl:allValuesFrom :Mapping ;
                owl:onProperty :hasMapping
              ] .

:valuesTransformedBy
      a       owl:ObjectProperty ;
      rdfs:label "values transformed by"@en .

:ObjectPropertyMapping
      a       owl:Class ;
      rdfs:comment "An entity specialized from Mapping than indicates the relation between a given key (provided as structure data in an online resource) and the OWL object property to which the values should be mapped and optionally the rdfs class or classes that the target instances belong to."@en ;
      rdfs:label "Object property mapping"@en ;
      rdfs:subClassOf :Mapping ;
      rdfs:subClassOf
              [ a       owl:Restriction ;
                owl:maxQualifiedCardinality
                        "1"^^xsd:nonNegativeInteger ;
                owl:onClass <http://iot.linkeddata.es/def/wot#ThingDescription> ;
                owl:onProperty :valuesTransformedBy
              ] ;
      rdfs:subClassOf
              [ a       owl:Restriction ;
                owl:allValuesFrom rdfs:Class ;
                owl:onProperty :targetClass
              ] ;
      rdfs:subClassOf
              [ a       owl:Restriction ;
                owl:allValuesFrom owl:ObjectProperty ;
                owl:onProperty :predicate
              ] .

rdfs:Datatype
      a       owl:Class ;
      rdfs:isDefinedBy rdfs: .

:key  a       owl:DatatypeProperty ;
      rdfs:comment "Field to be mapped from the endpoint"@en ;
      rdfs:domain :Mapping ;
      rdfs:label "key"@en ;
      rdfs:range xsd:string .

:predicate
      a       owl:ObjectProperty ;
      rdfs:comment "Link from a mapping an the property or properties to which the key should be mapped to. The property could be RDF properties or OWL object or datatype properties."@en ;
      rdfs:label "predicate"@en .

dcterms:contributor
      a       owl:AnnotationProperty .

:hasMapping
      a       owl:ObjectProperty ;
      rdfs:comment "Link between the access mappings to specific mappings."@en ;
      rdfs:domain :AccessMapping ;
      rdfs:label "has mapping"@en ;
      rdfs:range :Mapping .

owl:ObjectProperty
      a       owl:Class ;
      rdfs:isDefinedBy owl: ;
      rdfs:subClassOf rdf:Property .

:targetClass
      a       owl:ObjectProperty ;
      rdfs:domain :ObjectPropertyMapping ;
      rdfs:label "target class"@en ;
      rdfs:range rdfs:Class .

rdfs:Class
      a       owl:Class ;
      rdfs:isDefinedBy rdfs: .

:exposes
      a       owl:ObjectProperty ;
      rdfs:comment "Link from a thing description to the endpoints in which it exposes information"@en ;
      rdfs:domain <http://iot.linkeddata.es/def/wot#ThingDescription> ;
      rdfs:label "exposes"@en ;
      rdfs:range <http://iot.linkeddata.es/def/wot#Endpoint> .

rdf:Property
      a       owl:Class ;
      rdfs:isDefinedBy rdf: .

:DatatypePropertyMapping
      a       owl:Class ;
      rdfs:comment "An entity specialized from Mapping than indicates the relation between a given key (provided as structure data in an online resource) and the OWL datatype property to which the values should be mapped and optionally the rdfs datatype in which the values are expressed."@en ;
      rdfs:label "Datatype property mapping"@en ;
      rdfs:subClassOf :Mapping ;
      rdfs:subClassOf
              [ a       owl:Restriction ;
                owl:allValuesFrom owl:DatatypeProperty ;
                owl:onProperty :predicate
              ] ;
      rdfs:subClassOf
              [ a       owl:Restriction ;
                owl:allValuesFrom rdfs:Datatype ;
                owl:onProperty :targetDatatype
              ] .
